HybridVerifVecs/hs_vc_examples.thy
@@ -1,10 +1,17 @@
+(*  Title:       Examples of hybrid systems verifications
+    Author:      Jonathan Julián Huerta y Munive, 2019
+    Maintainer:  Jonathan Julián Huerta y Munive <jjhuertaymunive1@sheffield.ac.uk>
+*)
+
+subsection \<open> Examples \<close>
+
+text \<open> We prove partial correctness specifications of some hybrid systems with our 
+verification components.\<close>
+
 theory hs_vc_examples
   imports hs_prelims_matrices hs_vc_spartan
 
 begin
-
-
-subsection\<open> Examples \<close>
 
 text\<open> Preliminary preparation for the examples.\<close>
 
@@ -41,9 +48,6 @@ abbreviation val_p :: "real^program_vars \<Rightarrow> string \<Rightarrow> real
 
 lemma "CARD(2) = CARD(program_vars)"
   unfolding number_of_program_vars by simp
-
-lemma [simp]: "i \<noteq> (0::2) \<longrightarrow> i = 1" 
-  using exhaust_2 by fastforce
 
 lemma two_eq_zero: "(2::2) = 0" 
   by simp
@@ -403,13 +407,16 @@ lemmas wlp_temp_dyn = local_flow.fbox_g_ode_ivl[OF local_flow_temp_up _ UNIV_I]
 
 lemma thermostat: 
   assumes "a > 0" and "0 \<le> t" and "0 < Tmin" and "Tmax < L"
-  shows "(\<lambda>s. Tmin \<le> s\<downharpoonright>\<^sub>V''T'' \<and> s\<downharpoonright>\<^sub>V''T'' \<le> Tmax \<and> s\<downharpoonright>\<^sub>V''on''=0) \<le> fbox 
-  (LOOP (((\<restriction>\<^sub>V''t'')::=(\<lambda>s.0));((\<restriction>\<^sub>V''TT'')::=(\<lambda>s. s\<downharpoonright>\<^sub>V''T''));
-  (IF (\<lambda>s. s\<downharpoonright>\<^sub>V''on''=0 \<and> s\<downharpoonright>\<^sub>V''TT''\<le>Tmin + 1) THEN (\<restriction>\<^sub>V''on'' ::= (\<lambda>s.1)) ELSE 
-  (IF (\<lambda>s. s\<downharpoonright>\<^sub>V''on''=1 \<and> s\<downharpoonright>\<^sub>V''TT''\<ge>Tmax - 1) THEN (\<restriction>\<^sub>V''on'' ::= (\<lambda>s.0)) ELSE skip));
-  (IF (\<lambda>s. s\<downharpoonright>\<^sub>V''on''=0) THEN (x\<acute>=(f\<^sub>T a 0) & (\<lambda>s. s\<downharpoonright>\<^sub>V''t'' \<le> - (ln (Tmin/s\<downharpoonright>\<^sub>V''TT''))/a) on {0..t} UNIV @ 0) 
-  ELSE (x\<acute>=(f\<^sub>T a L) & (\<lambda>s. s\<downharpoonright>\<^sub>V''t'' \<le> - (ln ((L-Tmax)/(L-s\<downharpoonright>\<^sub>V''TT'')))/a) on {0..t} UNIV @ 0)) )
-  INV (\<lambda>s. Tmin \<le>s\<downharpoonright>\<^sub>V''T'' \<and> s\<downharpoonright>\<^sub>V''T''\<le>Tmax \<and> (s\<downharpoonright>\<^sub>V''on''=0 \<or> s\<downharpoonright>\<^sub>V''on''=1)))
+  shows "(\<lambda>s. Tmin \<le> s\<downharpoonright>\<^sub>V''T'' \<and> s\<downharpoonright>\<^sub>V''T'' \<le> Tmax \<and> s\<downharpoonright>\<^sub>V''on''=0) \<le> 
+  |LOOP 
+    \<comment> \<open>control\<close>
+    (((\<restriction>\<^sub>V''t'')::=(\<lambda>s.0));((\<restriction>\<^sub>V''TT'')::=(\<lambda>s. s\<downharpoonright>\<^sub>V''T''));
+    (IF (\<lambda>s. s\<downharpoonright>\<^sub>V''on''=0 \<and> s\<downharpoonright>\<^sub>V''TT''\<le>Tmin + 1) THEN (\<restriction>\<^sub>V''on'' ::= (\<lambda>s.1)) ELSE 
+    (IF (\<lambda>s. s\<downharpoonright>\<^sub>V''on''=1 \<and> s\<downharpoonright>\<^sub>V''TT''\<ge>Tmax - 1) THEN (\<restriction>\<^sub>V''on'' ::= (\<lambda>s.0)) ELSE skip));
+    \<comment> \<open>dynamics\<close>
+    (IF (\<lambda>s. s\<downharpoonright>\<^sub>V''on''=0) THEN (x\<acute>=(f\<^sub>T a 0) & (\<lambda>s. s\<downharpoonright>\<^sub>V''t'' \<le> - (ln (Tmin/s\<downharpoonright>\<^sub>V''TT''))/a) on {0..t} UNIV @ 0) 
+     ELSE (x\<acute>=(f\<^sub>T a L) & (\<lambda>s. s\<downharpoonright>\<^sub>V''t'' \<le> - (ln ((L-Tmax)/(L-s\<downharpoonright>\<^sub>V''TT'')))/a) on {0..t} UNIV @ 0)) )
+  INV (\<lambda>s. Tmin \<le>s\<downharpoonright>\<^sub>V''T'' \<and> s\<downharpoonright>\<^sub>V''T''\<le>Tmax \<and> (s\<downharpoonright>\<^sub>V''on''=0 \<or> s\<downharpoonright>\<^sub>V''on''=1))]
   (\<lambda>s. Tmin \<le> s$\<restriction>\<^sub>V''T'' \<and> s$\<restriction>\<^sub>V''T'' \<le> Tmax)"
   apply(rule fbox_loopI, simp_all add: wlp_temp_dyn[OF assms(1,2)] le_fun_def to_var_inject, safe)
   using temp_dyn_up_real_arith[OF assms(1) _ _ assms(4), of Tmin]
