HybridVerifVecs/hs_vc_spartan.thy
@@ -1,10 +1,19 @@
+(*  Title:       Verification components for hybrid systems 
+    Author:      Jonathan Julián Huerta y Munive, 2019
+    Maintainer:  Jonathan Julián Huerta y Munive <jjhuertaymunive1@sheffield.ac.uk>
+*)
+
+section \<open> Verification components for hybrid systems \<close>
+
+text \<open> A light-weight version of the verification components. We define the forward box 
+operator to compute weakest liberal preconditions (wlps) of hybrid programs. Then we 
+introduce three methods for verifying correctness specifications of the continuous 
+dynamics of a HS. \<close>
+
 theory hs_vc_spartan
   imports hs_prelims_dyn_sys
                         
 begin
-
-
-chapter \<open>Hybrid System Verification\<close>
 
 type_synonym 'a pred = "'a \<Rightarrow> bool"
 
@@ -15,7 +24,8 @@ notation Union ("\<mu>")
 
 abbreviation "skip \<equiv> (\<lambda>s. {s})"
 
-section \<open>Verification of regular programs\<close>
+
+subsection \<open>Verification of regular programs\<close>
 
 text \<open>First we add lemmas for computation of weakest liberal preconditions (wlps).\<close>
 
@@ -74,16 +84,10 @@ lemma fbox_if_then_else[simp]:
   "|IF T THEN X ELSE Y] Q = (\<lambda>s. (T s \<longrightarrow> ( |X] Q) s) \<and> (\<not> T s \<longrightarrow> ( |Y] Q) s))"
   unfolding fbox_def ifthenelse_def by auto
 
-lemma fbox_if_then_else_ge:
+lemma hoare_if_then_else:
   assumes "(\<lambda>s. P s \<and> T s) \<le> |X] Q"
     and "(\<lambda>s. P s \<and> \<not> T s) \<le> |Y] Q"
   shows "P \<le> |IF T THEN X ELSE Y] Q"
-  using assms unfolding fbox_def ifthenelse_def by auto
-
-lemma fbox_if_then_elseI:
-  assumes "T s \<longrightarrow> ( |X] Q) s"
-    and "\<not> T s \<longrightarrow> ( |Y] Q) s"
-  shows "( |IF T THEN X ELSE Y] Q) s"
   using assms unfolding fbox_def ifthenelse_def by auto
 
 text \<open>The final wlp we add is that of the finite iteration.\<close>
@@ -108,15 +112,13 @@ lemma kpower_inv:
   assumes "\<forall>s. I s \<longrightarrow> (\<forall>s'. s' \<in> F s \<longrightarrow> I s')" 
   shows "\<forall>s. I s \<longrightarrow> (\<forall>s'. s' \<in> (kpower F n s) \<longrightarrow> I s')"
   apply(clarsimp, induct n)
-  unfolding kpower_base apply simp
-  unfolding kpower_simp apply(simp add: kcomp_eq, clarsimp) 
+  unfolding kpower_base kpower_simp apply(simp_all add: kcomp_eq, clarsimp) 
   apply(subgoal_tac "I y", simp)
   using assms by blast
 
 lemma kstar_inv: "I \<le> |F] I \<Longrightarrow> I \<le> |F\<^sup>*] I"
   unfolding kleene_star_def fbox_def apply clarsimp
   apply(unfold le_fun_def, subgoal_tac "\<forall>x. I x \<longrightarrow> (\<forall>s'. s' \<in> F x \<longrightarrow> I s')")
-  apply(thin_tac "\<forall>x. I x \<le> (\<forall>s'. s' \<in> F x \<longrightarrow> I s')")
   using kpower_inv[of I F] by blast simp
 
 lemma fbox_kstarI:
@@ -139,10 +141,9 @@ lemma fbox_loopI: "P \<le> I \<Longrightarrow> I \<le> Q \<Longrightarrow> I \<l
   unfolding loopi_def using fbox_kstarI[of "P"] by simp
 
 
-section \<open>Verification of hybrid programs\<close>
+subsection \<open>Verification of hybrid programs\<close>
 
-
-subsection \<open>Verification by providing evolution\<close>
+text \<open>Verification by providing evolution\<close>
 
 definition g_evol :: "(('a::ord) \<Rightarrow> 'b \<Rightarrow> 'b) \<Rightarrow> 'b pred \<Rightarrow> 'a set \<Rightarrow> ('b \<Rightarrow> 'b set)" ("EVOL")
   where "EVOL \<phi> G T = (\<lambda>s. g_orbit (\<lambda>t. \<phi> t s) G T)"
@@ -152,8 +153,7 @@ lemma fbox_g_evol[simp]:
   shows "|EVOL \<phi> G T] Q = (\<lambda>s. (\<forall>t\<in>T. (\<forall>\<tau>\<in>down T t. G (\<phi> \<tau> s)) \<longrightarrow> Q (\<phi> t s)))"
   unfolding g_evol_def g_orbit_eq fbox_def by auto
 
-
-subsection \<open>Verification by providing solutions\<close>
+text \<open>Verification by providing solutions\<close>
 
 lemma fbox_g_orbital: "|x\<acute>=f & G on T S @ t\<^sub>0] Q = 
   (\<lambda>s. \<forall>X\<in>Sols (\<lambda>t. f) T S t\<^sub>0 s. \<forall>t\<in>T. (\<forall>\<tau>\<in>down T t. G (X \<tau>)) \<longrightarrow> Q (X t))"
@@ -189,8 +189,7 @@ lemma fbox_orbit: "|\<gamma>\<^sup>\<phi>] Q = (\<lambda>s. s \<in> S \<longrigh
 
 end
 
-
-subsection\<open> Verification with differential invariants \<close>
+text \<open> Verification with differential invariants \<close>
 
 definition g_ode_inv :: "(('a::banach)\<Rightarrow>'a) \<Rightarrow> 'a pred \<Rightarrow> real set \<Rightarrow> 'a set \<Rightarrow> 
   real \<Rightarrow> 'a pred \<Rightarrow> ('a \<Rightarrow> 'a set)" ("(1x\<acute>=_ & _ on _ _ @ _ DINV _ )") 
@@ -212,6 +211,28 @@ lemma fbox_diff_inv[simp]:
   "(I \<le> |x\<acute>=f & G on T S @ t\<^sub>0] I) = diff_invariant I f T S t\<^sub>0 G"
   by (auto simp: diff_invariant_def ivp_sols_def fbox_def g_orbital_eq)
 
+lemma diff_inv_guard_ignore:
+  assumes "I \<le> |x\<acute>= f & (\<lambda>s. True) on T S @ t\<^sub>0] I"
+  shows "I \<le> |x\<acute>= f & G on T S @ t\<^sub>0] I"
+  using assms unfolding fbox_diff_inv diff_invariant_eq by auto
+
+context local_flow
+begin
+
+lemma fbox_diff_inv_eq: "diff_invariant I f T S 0 (\<lambda>s. True) = 
+  ((\<lambda>s. s \<in> S \<longrightarrow> I s) = |x\<acute>= f & (\<lambda>s. True) on T S @ 0] (\<lambda>s. s \<in> S \<longrightarrow> I s))"
+  unfolding fbox_diff_inv[symmetric] fbox_g_orbital le_fun_def fun_eq_iff
+  using init_time apply(clarsimp simp: subset_eq ivp_sols_def)
+  apply(safe, force, force)
+   apply(subst ivp(2)[symmetric], simp)
+   apply(erule_tac x="\<lambda>t. \<phi> t x" in allE)
+  using in_domain has_vderiv_on_domain ivp(2) init_time by auto
+
+lemma diff_inv_eq_inv_set: "diff_invariant I f T S 0 (\<lambda>s. True) = (\<forall>s. I s \<longrightarrow> \<gamma>\<^sup>\<phi> s \<subseteq> {s. I s})"
+  unfolding diff_inv_eq_inv_set orbit_def by simp
+
+end
+
 lemma fbox_g_odei: "P \<le> I \<Longrightarrow> I \<le> |x\<acute>= f & G on T S @ t\<^sub>0] I \<Longrightarrow> (\<lambda>s. I s \<and> G s) \<le> Q \<Longrightarrow> 
   P \<le> |x\<acute>= f & G on T S @ t\<^sub>0 DINV I] Q"
   unfolding g_ode_inv_def apply(rule_tac b="|x\<acute>= f & G on T S @ t\<^sub>0] I" in order.trans)
@@ -219,10 +240,131 @@ lemma fbox_g_odei: "P \<le> I \<Longrightarrow> I \<le> |x\<acute>= f & G on T S
   apply(subst fbox_g_orbital_guard, simp)
   by (rule fbox_iso, force)
 
+
+subsection \<open> Derivation of the rules of dL \<close>
+
+text \<open> We derive domain specific rules of differential dynamic logic (dL). First we present a 
+generalised version, then we show the rules as instances of the general ones.\<close>
+
+lemma diff_solve_axiom: 
+  fixes c::"'a::{heine_borel, banach}"
+  assumes "0 \<in> T" and "is_interval T" "open T"
+  shows "|x\<acute>=(\<lambda>s. c) & G on T UNIV @ 0] Q = 
+  (\<lambda>s. \<forall>t\<in>T. (\<P> (\<lambda>\<tau>. s + \<tau> *\<^sub>R c) (down T t) \<subseteq> {s. G s}) \<longrightarrow> Q (s + t *\<^sub>R c))"
+  apply(subst local_flow.fbox_g_ode[of "\<lambda>s. c" _ _ "(\<lambda>t s. s + t *\<^sub>R c)"])
+  using line_is_local_flow assms by auto
+
+lemma diff_solve_rule:
+  assumes "local_flow f T UNIV \<phi>"
+    and "\<forall>s. P s \<longrightarrow> (\<forall> t\<in>T. (\<P> (\<lambda>t. \<phi> t s) (down T t) \<subseteq> {s. G s}) \<longrightarrow> Q (\<phi> t s))"
+  shows "P \<le> |x\<acute>= f & G on T UNIV @ 0] Q"
+  using assms by(subst local_flow.fbox_g_ode) auto
+
+lemma diff_weak_axiom: "|x\<acute>= f & G on T S @ t\<^sub>0] Q = |x\<acute>= f & G on T S @ t\<^sub>0] (\<lambda>s. G s \<longrightarrow> Q s)"
+  unfolding fbox_g_orbital image_def by force
+  
+lemma diff_weak_rule: "G \<le> Q \<Longrightarrow> P \<le> |x\<acute>= f & G on T S @ t\<^sub>0] Q"
+  by(auto intro: g_orbitalD simp: le_fun_def g_orbital_eq fbox_def)
+
+lemma fbox_g_orbital_eq_univD:
+  assumes "|x\<acute>= f & G on T S @ t\<^sub>0] C = (\<lambda>s. True)" 
+    and "\<forall>\<tau>\<in>(down T t). x \<tau> \<in> (x\<acute>= f & G on T S @ t\<^sub>0) s"
+  shows "\<forall>\<tau>\<in>(down T t). C (x \<tau>)"
+proof
+  fix \<tau> assume "\<tau> \<in> (down T t)"
+  hence "x \<tau> \<in> (x\<acute>= f & G on T S @ t\<^sub>0) s" 
+    using assms(2) by blast
+  also have "\<forall>s'. s' \<in> (x\<acute>= f & G on T S @ t\<^sub>0) s \<longrightarrow> C s'"
+    using assms(1) unfolding fbox_def by meson 
+  ultimately show "C (x \<tau>)" by blast
+qed
+
+lemma diff_cut_axiom:
+  assumes Thyp: "is_interval T" "t\<^sub>0 \<in> T"
+    and "|x\<acute>= f & G on T S @ t\<^sub>0] C = (\<lambda>s. True)"
+  shows "|x\<acute>= f & G on T S @ t\<^sub>0] Q = |x\<acute>= f & (\<lambda>s. G s \<and> C s) on T S @ t\<^sub>0] Q"
+proof(rule_tac f="\<lambda> x. |x] Q" in HOL.arg_cong, rule ext, rule subset_antisym)
+  fix s 
+  {fix s' assume "s' \<in> (x\<acute>= f & G on T S @ t\<^sub>0) s"
+    then obtain \<tau>::real and X where x_ivp: "X \<in> Sols (\<lambda>t. f) T S t\<^sub>0 s" 
+      and "X \<tau> = s'" and "\<tau> \<in> T" and guard_x:"\<P> X (down T \<tau>) \<subseteq> {s. G s}"
+      using g_orbitalD[of s' "f" G T S t\<^sub>0 s]  by blast
+    have "\<forall>t\<in>(down T \<tau>). \<P> X (down T t) \<subseteq> {s. G s}"
+      using guard_x by (force simp: image_def)
+    also have "\<forall>t\<in>(down T \<tau>). t \<in> T"
+      using \<open>\<tau> \<in> T\<close> Thyp closed_segment_subset_interval by auto
+    ultimately have "\<forall>t\<in>(down T \<tau>). X t \<in> (x\<acute>= f & G on T S @ t\<^sub>0) s"
+      using g_orbitalI[OF x_ivp] by (metis (mono_tags, lifting))
+    hence "\<forall>t\<in>(down T \<tau>). C (X t)" 
+      using assms(3) unfolding fbox_def by meson
+    hence "s' \<in> (x\<acute>= f & (\<lambda>s. G s \<and> C s) on T S @ t\<^sub>0) s"
+      using g_orbitalI[OF x_ivp \<open>\<tau> \<in> T\<close>] guard_x \<open>X \<tau> = s'\<close> by fastforce}
+  thus "(x\<acute>= f & G on T S @ t\<^sub>0) s \<subseteq> (x\<acute>= f & (\<lambda>s. G s \<and> C s) on T S @ t\<^sub>0) s"
+    by blast
+next show "\<And>s. (x\<acute>= f & (\<lambda>s. G s \<and> C s) on T S @ t\<^sub>0) s \<subseteq> (x\<acute>= f & G on T S @ t\<^sub>0) s" 
+    by (auto simp: g_orbital_eq)
+qed
+
+lemma diff_cut_rule:
+  assumes Thyp: "is_interval T" "t\<^sub>0 \<in> T"
+    and fbox_C: "P \<le> |x\<acute>= f & G on T S @ t\<^sub>0] C"
+    and fbox_Q: "P \<le> |x\<acute>= f & (\<lambda>s. G s \<and> C s) on T S @ t\<^sub>0] Q"
+  shows "P \<le> |x\<acute>= f & G on T S @ t\<^sub>0] Q"
+proof(subst fbox_def, subst g_orbital_eq, clarsimp)
+  fix t::real and X::"real \<Rightarrow> 'a" and s assume "P s" and "t \<in> T"
+    and x_ivp:"X \<in> Sols (\<lambda>t. f) T S t\<^sub>0 s" 
+    and guard_x:"\<forall>\<tau>. \<tau> \<in> T \<and> \<tau> \<le> t \<longrightarrow> G (X \<tau>)"
+  have "\<forall>\<tau>\<in>(down T t). X \<tau> \<in> (x\<acute>= f & G on T S @ t\<^sub>0) s"
+    using g_orbitalI[OF x_ivp] guard_x by auto
+  hence "\<forall>\<tau>\<in>(down T t). C (X \<tau>)" 
+    using fbox_C \<open>P s\<close> by (subst (asm) fbox_def, auto)
+  hence "X t \<in> (x\<acute>= f & (\<lambda>s. G s \<and> C s) on T S @ t\<^sub>0) s"
+    using guard_x \<open>t \<in> T\<close> by (auto intro!: g_orbitalI x_ivp)
+  thus "Q (X t)"
+    using \<open>P s\<close> fbox_Q by (subst (asm) fbox_def) auto
+qed
+
+text \<open>The rules of dL\<close>
+
 abbreviation g_global_orbit ::"(('a::banach)\<Rightarrow>'a) \<Rightarrow> 'a pred \<Rightarrow> 'a \<Rightarrow> 'a set" 
   ("(1x\<acute>=_ & _)") where "(x\<acute>=f & G) \<equiv> (x\<acute>=f & G on UNIV UNIV @ 0)"
 
 abbreviation g_global_ode_inv ::"(('a::banach)\<Rightarrow>'a) \<Rightarrow> 'a pred \<Rightarrow> 'a pred \<Rightarrow> 'a \<Rightarrow> 'a set" 
   ("(1x\<acute>=_ & _ DINV _)") where "(x\<acute>=f & G DINV I) \<equiv> (x\<acute>=f & G on UNIV UNIV @ 0 DINV I)"
+
+lemma solve:
+  assumes "local_flow f UNIV UNIV \<phi>"
+    and "\<forall>s. P s \<longrightarrow> (\<forall>t. (\<forall>\<tau>\<le>t. G (\<phi> \<tau> s)) \<longrightarrow> Q (\<phi> t s))"
+  shows "P \<le> |x\<acute>= f & G] Q"
+  apply(rule diff_solve_rule[OF assms(1)])
+  using assms(2) by simp
+
+lemma DS: 
+  fixes c::"'a::{heine_borel, banach}"
+  shows "|x\<acute>=(\<lambda>s. c) & G] Q = (\<lambda>x. \<forall>t. (\<forall>\<tau>\<le>t. G (x + \<tau> *\<^sub>R c)) \<longrightarrow> Q (x + t *\<^sub>R c))"
+  by (subst diff_solve_axiom[of UNIV]) auto
+
+lemma DW: "|x\<acute>= f & G] Q = |x\<acute>= f & G] (\<lambda>s. G s \<longrightarrow> Q s)"
+  by (rule diff_weak_axiom)
+  
+lemma dW: "G \<le> Q \<Longrightarrow> P \<le> |x\<acute>= f & G] Q"
+  by (rule diff_weak_rule)
+
+lemma DC:
+  assumes "|x\<acute>= f & G] C = (\<lambda>s. True)"
+  shows "|x\<acute>= f & G] Q = |x\<acute>= f & (\<lambda>s. G s \<and> C s)] Q"
+  by (rule diff_cut_axiom) (auto simp: assms)
+
+lemma dC:
+  assumes "P \<le> |x\<acute>= f & G] C"
+    and "P \<le> |x\<acute>= f & (\<lambda>s. G s \<and> C s)] Q"
+  shows "P \<le> |x\<acute>= f & G] Q"
+  apply(rule diff_cut_rule)
+  using assms by auto
+
+lemma dI:
+  assumes "P \<le> I" and "diff_invariant I f UNIV UNIV 0 G" and "I \<le> Q"
+  shows "P \<le> |x\<acute>= f & G] Q"
+  by (rule fbox_g_orbital_inv[OF assms(1) _ assms(3)]) (simp add: assms(2))
 
 end
